Fixed up stack and closure

04Stack/Stack.thy
@@ -1,5 +1,5 @@
 theory Stack
-  imports "../03Debruijn/DebruijnIndices" "../00Utils/Iteration"
+  imports "../03Debruijn/LetFloating" "../00Utils/Iteration"
 begin
 
 section \<open>Stack Evaluation\<close>
@@ -18,14 +18,13 @@ take the opportunity to get rid of explicitly testing expressions for being valu
 
 text \<open>There are only three things to search through, the left and right subexpressions of an \<open>App\<^sub>d\<close>, 
 and the left subexpression of a \<open>Let\<^sub>d\<close>, so there is a frame for each, recording our position in the 
-search. The \<open>FPop\<^sub>k\<close> and \<open>FReturn\<^sub>k\<close> frames are not strictly necessary for this stage, but recording 
-each time we change the implicit evaluation environment will make future stages possible.\<close>
+search. The \<open>FReturn\<^sub>k\<close> frame is not strictly necessary for this stage, but recording each time we 
+change the implicit evaluation environment will make future stages possible.\<close>
 
 datatype frame\<^sub>k = 
   FApp1\<^sub>k expr\<^sub>d
   | FApp2\<^sub>k expr\<^sub>d
   | FLet\<^sub>k expr\<^sub>d
-  | FPop\<^sub>k
   | FReturn\<^sub>k
 
 text \<open>Typing a stack is simple. Since the stack represents, in effect, an expression with a hole in 
@@ -33,34 +32,61 @@ it for the subexpression under evaluation, it takes a type for that inner expres
 type for the type of the stack and expression together. Since the stack has no binders and is always
 created from a closed expression, we do not need a typing context, either. Note that since we only 
 ever search the left side of an \<open>App\<^sub>d\<close> when the right is a value, we enforce that the expression 
-stored in a \<open>FApp2\<^sub>k\<close> frame must be a value too.\<close>
+stored in a \<open>FApp2\<^sub>k\<close> frame must be a value too; we also retain our let-floating invariants. We are 
+also able to guarantee that there is always an \<open>FReturn\<^sub>c\<close> frame above an \<open>FLet\<^sub>c\<close> because all our 
+expressions have been let-floated - indeed, this property is precisely what it means to be 
+let-floated in a stack context\<close>
+
+fun return_headed\<^sub>k :: "frame\<^sub>k list \<Rightarrow> bool" where
+  "return_headed\<^sub>k (FReturn\<^sub>k # s) = True"
+| "return_headed\<^sub>k s = False"
+
+lemma return_headed_elim [dest]: "return_headed\<^sub>k s \<Longrightarrow> \<exists>s'. s = FReturn\<^sub>k # s'"
+  by (cases s rule: return_headed\<^sub>k.cases) simp_all
+
+lemma return_headed_append [simp]: "return_headed\<^sub>k (s @ s') = 
+    (return_headed\<^sub>k s \<or> (s = [] \<and> return_headed\<^sub>k s'))"
+  by (cases s rule: return_headed\<^sub>k.cases) simp_all
 
 inductive typing_stack\<^sub>k :: "frame\<^sub>k list \<Rightarrow> ty \<Rightarrow> ty \<Rightarrow> bool" (infix ":\<^sub>k _ \<rightarrow>" 50) where
   tcs\<^sub>k_nil [simp]: "[] :\<^sub>k t \<rightarrow> t"
-| tcs\<^sub>k_cons_app1 [simp]: "[] \<turnstile>\<^sub>d e : t\<^sub>1 \<Longrightarrow> s :\<^sub>k t\<^sub>2 \<rightarrow> t \<Longrightarrow> FApp1\<^sub>k e # s :\<^sub>k Arrow t\<^sub>1 t\<^sub>2 \<rightarrow> t"
-| tcs\<^sub>k_cons_app2 [simp]: "[] \<turnstile>\<^sub>d e : Arrow t\<^sub>1 t\<^sub>2 \<Longrightarrow> value\<^sub>d e \<Longrightarrow> s :\<^sub>k t\<^sub>2 \<rightarrow> t \<Longrightarrow> 
+| tcs\<^sub>k_cons_app1 [simp]: "[] \<turnstile>\<^sub>d e : t\<^sub>1 \<Longrightarrow> let_floated\<^sub>d e \<Longrightarrow> let_free\<^sub>d e \<Longrightarrow> s :\<^sub>k t\<^sub>2 \<rightarrow> t \<Longrightarrow> 
+    FApp1\<^sub>k e # s :\<^sub>k Arrow t\<^sub>1 t\<^sub>2 \<rightarrow> t"
+| tcs\<^sub>k_cons_app2 [simp]: "[] \<turnstile>\<^sub>d e : Arrow t\<^sub>1 t\<^sub>2 \<Longrightarrow> let_floated\<^sub>d e \<Longrightarrow> value\<^sub>d e \<Longrightarrow> s :\<^sub>k t\<^sub>2 \<rightarrow> t \<Longrightarrow> 
     FApp2\<^sub>k e # s :\<^sub>k t\<^sub>1 \<rightarrow> t"
-| tcs\<^sub>k_cons_let [simp]: "[t\<^sub>1] \<turnstile>\<^sub>d e : t\<^sub>2 \<Longrightarrow> s :\<^sub>k t\<^sub>2 \<rightarrow> t \<Longrightarrow> FLet\<^sub>k e # s :\<^sub>k t\<^sub>1 \<rightarrow> t"
-| tcs\<^sub>k_cons_pop [simp]: "s :\<^sub>k t' \<rightarrow> t \<Longrightarrow> FPop\<^sub>k # s :\<^sub>k t' \<rightarrow> t"
+| tcs\<^sub>k_cons_let [simp]: "[t\<^sub>1] \<turnstile>\<^sub>d e : t\<^sub>2 \<Longrightarrow> let_floated\<^sub>d e \<Longrightarrow> s :\<^sub>k t\<^sub>2 \<rightarrow> t \<Longrightarrow> return_headed\<^sub>k s \<Longrightarrow>
+    FLet\<^sub>k e # s :\<^sub>k t\<^sub>1 \<rightarrow> t"
 | tcs\<^sub>k_cons_ret [simp]: "s :\<^sub>k t' \<rightarrow> t \<Longrightarrow> FReturn\<^sub>k # s :\<^sub>k t' \<rightarrow> t"
 
 inductive_cases [elim]: "[] :\<^sub>k t' \<rightarrow> t"
 inductive_cases [elim]: "FApp1\<^sub>k e # s :\<^sub>k t' \<rightarrow> t"
 inductive_cases [elim]: "FApp2\<^sub>k e # s :\<^sub>k t' \<rightarrow> t"
 inductive_cases [elim]: "FLet\<^sub>k e # s :\<^sub>k t' \<rightarrow> t"
-inductive_cases [elim]: "FPop\<^sub>k # s :\<^sub>k t' \<rightarrow> t"
 inductive_cases [elim]: "FReturn\<^sub>k # s :\<^sub>k t' \<rightarrow> t"
 
-lemma tc_stack\<^sub>k_append [simp]: "s @ s' :\<^sub>k t' \<rightarrow> t \<Longrightarrow> \<exists>t''. (s :\<^sub>k t' \<rightarrow> t'') \<and> (s' :\<^sub>k t'' \<rightarrow> t)"
+lemma tc_stack\<^sub>k_append [simp]: "s @ s' :\<^sub>k t' \<rightarrow> t \<Longrightarrow> \<not> return_headed\<^sub>k s' \<Longrightarrow> 
+  \<exists>t''. (s :\<^sub>k t' \<rightarrow> t'') \<and> (s' :\<^sub>k t'' \<rightarrow> t)"
 proof (induction s arbitrary: t')
   case (Cons f s)
   thus ?case 
   proof (induction f)
     case (FApp2\<^sub>k e)
-    then obtain t\<^sub>2 where X: "([] \<turnstile>\<^sub>d e : Arrow t' t\<^sub>2) \<and> value\<^sub>d e \<and> (s @ s' :\<^sub>k t\<^sub>2 \<rightarrow> t)" by auto
+    then obtain t\<^sub>2 where X: "([] \<turnstile>\<^sub>d e : Arrow t' t\<^sub>2) \<and> let_floated\<^sub>d e \<and> let_free\<^sub>d e \<and> value\<^sub>d e \<and> 
+      (s @ s' :\<^sub>k t\<^sub>2 \<rightarrow> t)" by auto
     with FApp2\<^sub>k obtain t'' where "(s :\<^sub>k t\<^sub>2 \<rightarrow> t'') \<and> (s' :\<^sub>k t'' \<rightarrow> t)" by blast
     moreover with X have "FApp2\<^sub>k e # s :\<^sub>k t' \<rightarrow> t''" by fastforce
     ultimately show ?case by blast
+  next
+    case (FLet\<^sub>k e)
+    then obtain tt where X: "([t'] \<turnstile>\<^sub>d e : tt) \<and> let_floated\<^sub>d e" and "s @ s' :\<^sub>k tt \<rightarrow> t"
+      and S: "return_headed\<^sub>k (s @ s')" by fastforce
+    with FLet\<^sub>k obtain t'' where T: "(s :\<^sub>k tt \<rightarrow> t'') \<and> s' :\<^sub>k t'' \<rightarrow> t" by fastforce
+    with S FLet\<^sub>k show ?case
+    proof (cases s)
+      case (Cons f s)
+      with S X T Cons have "FLet\<^sub>k e # FReturn\<^sub>k # s :\<^sub>k t' \<rightarrow> t''" by auto
+      with S T Cons show ?thesis by auto
+    qed simp_all
   qed force+
 qed force+
 
@@ -77,7 +103,8 @@ text \<open>Typechecking a full state is equally simple. Again, we do not need a
 only ever evaluate closed expressions.\<close>
 
 inductive typing_state\<^sub>k :: "state\<^sub>k \<Rightarrow> ty \<Rightarrow> bool" (infix ":\<^sub>k" 50) where
-  tc_state\<^sub>k [simp]: "s :\<^sub>k t' \<rightarrow> t \<Longrightarrow> [] \<turnstile>\<^sub>d e : t' \<Longrightarrow> (b \<longrightarrow> value\<^sub>d e) \<Longrightarrow> S\<^sub>k b s e :\<^sub>k t"
+  tc_state\<^sub>k [simp]: "s :\<^sub>k t' \<rightarrow> t \<Longrightarrow> [] \<turnstile>\<^sub>d e : t' \<Longrightarrow> let_floated\<^sub>d e \<Longrightarrow> (b \<longrightarrow> value\<^sub>d e) \<Longrightarrow> 
+    let_free\<^sub>d e \<or> return_headed\<^sub>k s \<Longrightarrow> S\<^sub>k b s e :\<^sub>k t"
 
 inductive_cases [elim]: "S\<^sub>k b s e :\<^sub>k t"
 
@@ -92,9 +119,8 @@ inductive eval\<^sub>k :: "state\<^sub>k \<Rightarrow> state\<^sub>k \<Rightarro
 | ev\<^sub>k_app1 [simp]: "S\<^sub>k False s (App\<^sub>d e\<^sub>1 e\<^sub>2) \<leadsto>\<^sub>k S\<^sub>k False (FApp1\<^sub>k e\<^sub>2 # s) e\<^sub>1"
 | ev\<^sub>k_app2 [simp]: "S\<^sub>k True (FApp1\<^sub>k e\<^sub>2 # s) e\<^sub>1 \<leadsto>\<^sub>k S\<^sub>k False (FApp2\<^sub>k e\<^sub>1 # s) e\<^sub>2"
 | ev\<^sub>k_app3 [simp]: "S\<^sub>k True (FApp2\<^sub>k (Lam\<^sub>d t e\<^sub>1) # s) e\<^sub>2 \<leadsto>\<^sub>k S\<^sub>k False (FReturn\<^sub>k # s) (subst\<^sub>d 0 e\<^sub>2 e\<^sub>1)"
-| ev\<^sub>k_let1 [simp]: "S\<^sub>k False s (Let\<^sub>d e\<^sub>1 e\<^sub>2) \<leadsto>\<^sub>k S\<^sub>k False (FLet\<^sub>k e\<^sub>2 # s) e\<^sub>1"
-| ev\<^sub>k_let2 [simp]: "S\<^sub>k True (FLet\<^sub>k e\<^sub>2 # s) e\<^sub>1 \<leadsto>\<^sub>k S\<^sub>k False (FPop\<^sub>k # s) (subst\<^sub>d 0 e\<^sub>1 e\<^sub>2)"
-| ev\<^sub>k_pop [simp]: "S\<^sub>k True (FPop\<^sub>k # s) e \<leadsto>\<^sub>k S\<^sub>k True s e"
+| ev\<^sub>k_let1 [simp]: "S\<^sub>k False (FReturn\<^sub>k # s) (Let\<^sub>d e\<^sub>1 e\<^sub>2) \<leadsto>\<^sub>k S\<^sub>k False (FLet\<^sub>k e\<^sub>2 # FReturn\<^sub>k # s) e\<^sub>1"
+| ev\<^sub>k_let2 [simp]: "S\<^sub>k True (FLet\<^sub>k e\<^sub>2 # FReturn\<^sub>k # s) e\<^sub>1 \<leadsto>\<^sub>k S\<^sub>k False (FReturn\<^sub>k # s) (subst\<^sub>d 0 e\<^sub>1 e\<^sub>2)"
 | ev\<^sub>k_ret [simp]: "S\<^sub>k True (FReturn\<^sub>k # s) e \<leadsto>\<^sub>k S\<^sub>k True s e"
 
 lemma eval\<^sub>k_under [simp]: "S\<^sub>k b s e \<leadsto>\<^sub>k S\<^sub>k b' s' e' \<Longrightarrow> S\<^sub>k b (s @ ss) e \<leadsto>\<^sub>k S\<^sub>k b' (s' @ ss) e'"
@@ -134,7 +160,8 @@ qed simp_all
 
 text \<open>From here, proving the safety theorems is straightforward:\<close>
 
-lemma eval\<^sub>k_from_nonvalue [simp]: "[] \<turnstile>\<^sub>d e : t \<Longrightarrow> \<exists>\<Sigma>'. S\<^sub>k False s e \<leadsto>\<^sub>k \<Sigma>'"
+lemma eval\<^sub>k_from_nonvalue [simp]: "[] \<turnstile>\<^sub>d e : t \<Longrightarrow> let_floated\<^sub>d e \<Longrightarrow> 
+  let_free\<^sub>d e \<or> return_headed\<^sub>k s \<Longrightarrow> \<exists>\<Sigma>'. S\<^sub>k False s e \<leadsto>\<^sub>k \<Sigma>'"
 proof (induction "[] :: ty list" e t rule: typing\<^sub>d.induct)
   case (tc\<^sub>d_const n)
   have "S\<^sub>k False s (Const\<^sub>d n) \<leadsto>\<^sub>k S\<^sub>k True s (Const\<^sub>d n)" by simp
@@ -149,8 +176,10 @@ next
   thus ?case by fastforce
 next
   case (tc\<^sub>d_let e\<^sub>1 t\<^sub>1 e\<^sub>2 t\<^sub>2)
-  have "S\<^sub>k False s (Let\<^sub>d e\<^sub>1 e\<^sub>2) \<leadsto>\<^sub>k S\<^sub>k False (FLet\<^sub>k e\<^sub>2 # s) e\<^sub>1" by simp
-  thus ?case by fastforce
+  then obtain s' where "s = FReturn\<^sub>k # s'" by auto
+  moreover have "S\<^sub>k False (FReturn\<^sub>k # s') (Let\<^sub>d e\<^sub>1 e\<^sub>2) \<leadsto>\<^sub>k S\<^sub>k False (FLet\<^sub>k e\<^sub>2 # FReturn\<^sub>k # s') e\<^sub>1" 
+    by simp
+  ultimately show ?case by fastforce
 qed simp_all
 
 lemma eval\<^sub>k_from_value [simp]: "s :\<^sub>k t' \<rightarrow> t \<Longrightarrow> [] \<turnstile>\<^sub>d e : t' \<Longrightarrow> value\<^sub>d e \<Longrightarrow> 
@@ -167,12 +196,9 @@ next
   ultimately show ?case by fastforce
 next
   case (tcs\<^sub>k_cons_let t\<^sub>1 e\<^sub>2 t\<^sub>2 s t)
-  hence "S\<^sub>k True (FLet\<^sub>k e\<^sub>2 # s) e \<leadsto>\<^sub>k S\<^sub>k False (FPop\<^sub>k # s) (subst\<^sub>d 0 e e\<^sub>2)" by simp
+  hence "S\<^sub>k True (FLet\<^sub>k e\<^sub>2 # s) e \<leadsto>\<^sub>k S\<^sub>k False s (subst\<^sub>d 0 e e\<^sub>2)" 
+    by (cases s rule: return_headed\<^sub>k.cases) simp_all
   then show ?case by fastforce
-next 
-  case (tcs\<^sub>k_cons_pop s t')
-  hence "S\<^sub>k True (FPop\<^sub>k # s) e \<leadsto>\<^sub>k S\<^sub>k True s e" by simp
-  thus ?case by fastforce
 next 
   case (tcs\<^sub>k_cons_ret s t')
   hence "S\<^sub>k True (FReturn\<^sub>k # s) e \<leadsto>\<^sub>k S\<^sub>k True s e" by simp
@@ -191,32 +217,36 @@ lemma final_no_eval\<^sub>k [simp]: "\<Sigma> \<leadsto>\<^sub>k \<Sigma>' \<Lon
 theorem preservation\<^sub>k [simp]: "\<Sigma> \<leadsto>\<^sub>k \<Sigma>' \<Longrightarrow> \<Sigma> :\<^sub>k t \<Longrightarrow> \<Sigma>' :\<^sub>k t"
 proof (induction \<Sigma> \<Sigma>' rule: eval\<^sub>k.induct)
   case (ev\<^sub>k_app1 s e\<^sub>1 e\<^sub>2)
-  then obtain t\<^sub>1 t\<^sub>2 where "s :\<^sub>k t\<^sub>2 \<rightarrow> t" and "[] \<turnstile>\<^sub>d e\<^sub>2 : t\<^sub>1" and X: "[] \<turnstile>\<^sub>d e\<^sub>1 : Arrow t\<^sub>1 t\<^sub>2" by blast
+  then obtain t\<^sub>1 t\<^sub>2 where "s :\<^sub>k t\<^sub>2 \<rightarrow> t" and "([] \<turnstile>\<^sub>d e\<^sub>2 : t\<^sub>1) \<and> let_free\<^sub>d e\<^sub>2 \<and> let_floated\<^sub>d e\<^sub>2" 
+    and X: "([] \<turnstile>\<^sub>d e\<^sub>1 : Arrow t\<^sub>1 t\<^sub>2) \<and> let_free\<^sub>d e\<^sub>1 \<and> let_floated\<^sub>d e\<^sub>1 \<and> (is_var\<^sub>d e\<^sub>1 \<or> value\<^sub>d e\<^sub>1)" 
+      by fastforce
   hence "FApp1\<^sub>k e\<^sub>2 # s :\<^sub>k Arrow t\<^sub>1 t\<^sub>2 \<rightarrow> t" by simp
   with X show ?case by simp
 next
   case (ev\<^sub>k_app2 e\<^sub>2 s e\<^sub>1)
-  then obtain t\<^sub>1 t\<^sub>2 where X: "[] \<turnstile>\<^sub>d e\<^sub>2 : t\<^sub>1" and "s :\<^sub>k t\<^sub>2 \<rightarrow> t" and "[] \<turnstile>\<^sub>d e\<^sub>1 : Arrow t\<^sub>1 t\<^sub>2" 
-   and "value\<^sub>d e\<^sub>1" by blast
-  with ev\<^sub>k_app2 have "FApp2\<^sub>k e\<^sub>1 # s :\<^sub>k t\<^sub>1 \<rightarrow> t" by simp
+  then obtain t\<^sub>1 t\<^sub>2 where X: "([] \<turnstile>\<^sub>d e\<^sub>2 : t\<^sub>1) \<and> let_free\<^sub>d e\<^sub>2 \<and> let_floated\<^sub>d e\<^sub>2" and "s :\<^sub>k t\<^sub>2 \<rightarrow> t" 
+   and "([] \<turnstile>\<^sub>d e\<^sub>1 : Arrow t\<^sub>1 t\<^sub>2) \<and> let_free\<^sub>d e\<^sub>1 \<and> let_floated\<^sub>d e\<^sub>1 \<and> value\<^sub>d e\<^sub>1" by fastforce
+  with ev\<^sub>k_app2 have "FApp2\<^sub>k e\<^sub>1 # s :\<^sub>k t\<^sub>1 \<rightarrow> t" by fastforce
   with X show ?case by simp
 next
   case (ev\<^sub>k_app3 t\<^sub>1 e\<^sub>1 s e\<^sub>2)
-  then obtain t\<^sub>2 where "[t\<^sub>1] \<turnstile>\<^sub>d e\<^sub>1 : t\<^sub>2" and X: "s :\<^sub>k t\<^sub>2 \<rightarrow> t" and "[] \<turnstile>\<^sub>d e\<^sub>2 : t\<^sub>1" by fastforce
-  hence "[] \<turnstile>\<^sub>d subst\<^sub>d 0 e\<^sub>2 e\<^sub>1 : t\<^sub>2" by simp
+  then obtain t\<^sub>2 where "([t\<^sub>1] \<turnstile>\<^sub>d e\<^sub>1 : t\<^sub>2) \<and> let_floated\<^sub>d e\<^sub>1" and X: "s :\<^sub>k t\<^sub>2 \<rightarrow> t" 
+    and "([] \<turnstile>\<^sub>d e\<^sub>2 : t\<^sub>1) \<and> let_floated\<^sub>d e\<^sub>2 \<and> value\<^sub>d e\<^sub>2" by fastforce
+  hence "([] \<turnstile>\<^sub>d subst\<^sub>d 0 e\<^sub>2 e\<^sub>1 : t\<^sub>2) \<and> let_floated\<^sub>d (subst\<^sub>d 0 e\<^sub>2 e\<^sub>1)" by fastforce
   moreover from X have "FReturn\<^sub>k # s :\<^sub>k t\<^sub>2 \<rightarrow> t" by simp
   ultimately show ?case by simp
 next
   case (ev\<^sub>k_let1 s e\<^sub>1 e\<^sub>2)
-  then obtain t\<^sub>1 t\<^sub>2 where "s :\<^sub>k t\<^sub>2 \<rightarrow> t" and X: "[] \<turnstile>\<^sub>d e\<^sub>1 : t\<^sub>1" and "[t\<^sub>1] \<turnstile>\<^sub>d e\<^sub>2 : t\<^sub>2" by fastforce
-  hence "FLet\<^sub>k e\<^sub>2 # s :\<^sub>k t\<^sub>1 \<rightarrow> t" by simp
+  then obtain t\<^sub>1 t\<^sub>2 where "s :\<^sub>k t\<^sub>2 \<rightarrow> t" and X: "([] \<turnstile>\<^sub>d e\<^sub>1 : t\<^sub>1) \<and> let_free\<^sub>d e\<^sub>1 \<and> let_floated\<^sub>d e\<^sub>1" 
+    and "([t\<^sub>1] \<turnstile>\<^sub>d e\<^sub>2 : t\<^sub>2) \<and> let_floated\<^sub>d e\<^sub>2" by fastforce
+  hence "FLet\<^sub>k e\<^sub>2 # FReturn\<^sub>k # s :\<^sub>k t\<^sub>1 \<rightarrow> t" by fastforce
   with X show ?case by simp
 next
   case (ev\<^sub>k_let2 e\<^sub>2 s e\<^sub>1)
-  then obtain t\<^sub>1 t\<^sub>2 where "[t\<^sub>1] \<turnstile>\<^sub>d e\<^sub>2 : t\<^sub>2" and X: "s :\<^sub>k t\<^sub>2 \<rightarrow> t" and "[] \<turnstile>\<^sub>d e\<^sub>1 : t\<^sub>1" and "value\<^sub>d e\<^sub>1" 
-    by fastforce
-  hence "[] \<turnstile>\<^sub>d subst\<^sub>d 0 e\<^sub>1 e\<^sub>2 : t\<^sub>2" by simp
-  moreover from X have "FPop\<^sub>k # s :\<^sub>k t\<^sub>2 \<rightarrow> t" by simp
+  then obtain t\<^sub>1 t\<^sub>2 where "([t\<^sub>1] \<turnstile>\<^sub>d e\<^sub>2 : t\<^sub>2) \<and> let_floated\<^sub>d e\<^sub>2" and X: "s :\<^sub>k t\<^sub>2 \<rightarrow> t" 
+    and "([] \<turnstile>\<^sub>d e\<^sub>1 : t\<^sub>1) \<and> let_floated\<^sub>d e\<^sub>1" and "value\<^sub>d e\<^sub>1" by fastforce
+  hence "([] \<turnstile>\<^sub>d subst\<^sub>d 0 e\<^sub>1 e\<^sub>2 : t\<^sub>2) \<and> let_floated\<^sub>d (subst\<^sub>d 0 e\<^sub>1 e\<^sub>2)" by fastforce
+  moreover from X have "FReturn\<^sub>k # s :\<^sub>k t\<^sub>2 \<rightarrow> t" by simp
   ultimately show ?case by simp
 qed fastforce+
 
@@ -244,9 +274,6 @@ next
   thus ?case by (induction rule: eval\<^sub>k.cases) simp_all
 next
   case (ev\<^sub>k_let2 e\<^sub>2 s e\<^sub>1)
-  thus ?case by (induction rule: eval\<^sub>k.cases) simp_all
-next 
-  case (ev\<^sub>k_pop s e)
   thus ?case by (induction rule: eval\<^sub>k.cases) simp_all
 next 
   case (ev\<^sub>k_ret s e)
